firmware/Hmac/Sha256ExampleProperties.v
@@ -1,0 +1,79 @@
+Require Import Coq.Strings.String.
+Require Import Coq.Lists.List.
+Require Import Coq.ZArith.ZArith.
+Require Import bedrock2.Array.
+Require Import bedrock2.Map.Separation.
+Require Import bedrock2.Map.SeparationLogic.
+Require Import bedrock2.ProgramLogic.
+Require Import bedrock2.Semantics.
+Require Import bedrock2.Syntax.
+Require Import bedrock2.WeakestPrecondition.
+Require Import bedrock2.WeakestPreconditionProperties.
+Require Import bedrock2.ZnWords.
+Require Import coqutil.Word.Interface.
+Require Import coqutil.Word.Properties.
+Require Import coqutil.Map.Interface.
+Require Import coqutil.Map.Properties.
+Require Import coqutil.Byte.
+Require Import Bedrock2Experiments.StateMachineSemantics.
+Require Import Bedrock2Experiments.Hmac.HmacSemantics.
+Require Import Bedrock2Experiments.Hmac.HmacProperties.
+Require Import Bedrock2Experiments.Hmac.Sha256Example.
+Import Syntax.Coercions List.ListNotations HList.
+Local Open Scope string_scope.
+Local Open Scope list_scope.
+Local Open Scope Z_scope.
+
+Section Proofs.
+  Context {word: word.word 32} {mem: map.map word byte}
+          {word_ok: word.ok word} {mem_ok: map.ok mem}.
+  Context {timing: timing}.
+
+  (* Plug in the right state machine parameters; typeclass inference struggles here *)
+  Local Notation execution := (execution (M:=hmac_state_machine)).
+
+  Notation bytearray := (array (mem := mem) ptsto (word.of_Z 1)).
+
+  Definition sha256_post(input_addr: word)(input: list byte)(digest_addr: word)(R: mem -> Prop)
+             (tr: trace)(m: mem)(rets: list word): Prop :=
+    rets = [] /\
+    execution tr (IDLE (sha256 input) (* digest has been read, but still in device *)
+                       {| hmac_done := false; (* done flag was already cleared *)
+                          intr_enable := word.of_Z 0;
+                          hmac_en := false;
+                          sha_en := true;
+                          swap_endian := true;
+                          swap_digest := false; |}) /\
+    (* digest has been stored at correct memory location: *)
+    (bytearray digest_addr (sha256 input) *
+    (* input and rest of memory unmodified: *)
+     bytearray input_addr input * R)%sep m.
+
+  Global Instance spec_of_sha256 : spec_of b2_sha256 :=
+    fun function_env =>
+      forall tr (m: mem) (R : mem -> Prop) (idlebuffer: list byte) (idleconfig: idle_data)
+             (input_addr input_len digest_addr: word) (input digest_trash: list byte),
+      Z.of_nat (length input) = word.unsigned input_len ->
+      Z.of_nat (length digest_trash) = 32 ->
+      input_addr <> word.of_Z 0 ->
+      digest_addr <> word.of_Z 0 ->
+      (bytearray input_addr input * bytearray digest_addr digest_trash * R)%sep m ->
+      execution tr (IDLE idlebuffer idleconfig) ->
+      call function_env b2_sha256 tr m [digest_addr; input_addr; input_len]
+           (sha256_post input_addr input digest_addr R).
+
+  Lemma sha256_correct :
+    program_logic_goal_for_function! b2_sha256.
+  Proof.
+    repeat straightline.
+    straightline_call. 1: ecancel_assumption. 1: eassumption.
+    repeat straightline.
+    straightline_call. 1: symmetry; eassumption. 1: assumption. 1: ecancel_assumption. 1: eassumption.
+    repeat straightline.
+    straightline_call. 1: eassumption. 1: assumption. 1: ecancel_assumption. 1: eassumption.
+    repeat straightline.
+    unfold sha256_post.
+    split; [reflexivity|]. split; [assumption|].
+    rewrite List.app_nil_l in *. ecancel_assumption.
+  Qed.
+End Proofs.
