silveroak-opentitan/Sha256End2End/Sha256ToCava.v
@@ -1,0 +1,87 @@
+Require Import Coq.Lists.List. Import ListNotations.
+Require Import Coq.ZArith.ZArith. Open Scope Z_scope.
+Require Import Coq.Strings.String. Open Scope string_scope.
+Require Import coqutil.Byte.
+Require Import coqutil.Word.Interface coqutil.Word.Properties.
+Require Import bedrock2.ZnWords.
+Require Import compiler.SeparationLogic.
+Require Import Bedrock2Experiments.RiscvMachineWithCavaDevice.ExtraRiscvMachine.
+Require Import Bedrock2Experiments.RiscvMachineWithCavaDevice.InternalMMIOMachine.
+Require Import Sha256End2End.CavaHmacDevice.
+Require Import Bedrock2Experiments.Hmac.Sha256ToRiscV.
+Require Import Bedrock2Experiments.RiscvMachineWithCavaDevice.Bedrock2ToCava.
+
+Definition binary: list byte := Eval compute in Pipeline.instrencode sha256_example_asm.
+
+(* TODO replace axiom from HmacSemantics with actual spec *)
+Definition sha256 := HmacSemantics.sha256.
+
+Axiom TODO: False.
+
+Theorem sha256_example_end2end_correct: forall p_functions p_call mH Rdata Rexec R (* <-? *)
+          (initialL: ExtraRiscvMachine hmac_device) digest_addr input_addr input_len
+          input output_placeholder sched,
+    -2^19 <= word.signed (word.sub p_functions p_call) < 2^19 ->
+    128 <= word.unsigned (word.sub stack_pastend stack_start) ->
+    word.unsigned (word.sub stack_pastend stack_start) mod 4 = 0 ->
+    word.unsigned p_functions mod 4 = 0 ->
+    word.unsigned p_call mod 4 = 0 ->
+    initialL.(getLog) = [] ->
+    machine_ok p_functions main_relative_pos stack_start stack_pastend binary p_call
+               p_call mH Rdata Rexec initialL ->
+    Z.of_nat (length input) = word.unsigned input_len ->
+    Z.of_nat (length output_placeholder) = 32 ->
+    input_addr <> word.of_Z 0 ->
+    digest_addr <> word.of_Z 0 ->
+    (scalar (word.of_Z digest_ptr) digest_addr *
+     scalar (word.of_Z msg_ptr) input_addr *
+     scalar (word.of_Z msg_len_ptr) input_len *
+     bytearray input_addr input * bytearray digest_addr output_placeholder * R)%sep mH ->
+    exists steps_remaining finalL mH',
+      run sched steps_remaining initialL = (Some tt, finalL) /\
+      machine_ok p_functions main_relative_pos stack_start stack_pastend binary p_call
+                 (word.add p_call (word.of_Z 4)) mH' Rdata Rexec finalL /\
+    (scalar (word.of_Z digest_ptr) digest_addr *
+     scalar (word.of_Z msg_ptr) input_addr *
+     scalar (word.of_Z msg_len_ptr) input_len *
+     bytearray input_addr input * bytearray digest_addr (sha256 input) * R)%sep mH' /\
+      finalL.(getLog) = initialL.(getLog) (* no external interactions happened *).
+Proof.
+  intros.
+  change binary with (Pipeline.instrencode sha256_example_asm).
+  refine (bedrock2_and_cava_system_correct
+            _ _ _ _ _ _ _ _ _ _ _ _ _ _ _ _ _ _ _ _ _ _ _ _ _ _ _ _ _ _ _ _ _);
+    try eassumption.
+  { exact funcs_valid. }
+  { apply List.dedup_NoDup_iff with (aeqb_spec:=String.eqb_spec). reflexivity. }
+  { exact sha256_compile_result_eq. }
+  { (* check that the compiler emitted valid instructions: *)
+    repeat (apply Forall_cons || apply Forall_nil).
+    all: try (vm_compute; intuition discriminate). }
+  { let p := eval cbv in main_relative_pos in change main_relative_pos with p. Lia.lia. }
+  { instantiate (2 := "main"). reflexivity. }
+  { reflexivity. }
+  { vm_compute. discriminate. }
+  { refine (WeakestPreconditionProperties.Proper_cmd _ _ _ _ _ _ _ _ _ _ _).
+    1: eapply WeakestPreconditionProperties.Proper_call.
+    2: {
+      eapply main_correct with (idlebuffer := List.repeat Byte.x00 32); cycle -2; try eassumption.
+      match goal with
+      | H: ?t = ?t' |- _ ?t'' _ => replace t'' with t' by exact H
+      end.
+      cbn.
+      case TODO.
+      (* make length of digest buffer match, and how to make it unique to satisfy Cava connection? *)
+    }
+    unfold Sha256ExampleProperties.sha256_post.
+    repeat intro. Tactics.logical_simplify. Tactics.ssplit.
+    { unfold sha256. ecancel_assumption. }
+    eexists. split; [eassumption|]. cbn. case TODO.
+    (* here, IDLE state with a sha in its digest_buffer must be an initial state *)
+  }
+  Unshelve. case TODO. (* initial state will be determined *)
+Qed.
+
+(* Goal: bring this list down to only standard axioms like functional and propositional extensionality
+Print Assumptions sha256_example_end2end_correct.
+ *)
